spec/abstract/ARM/ArchTcb_A.thy
@@ -25,5 +25,12 @@ definition
 where
   "arch_tcb_set_ipc_buffer target ptr \<equiv> as_user target $ set_register TPIDRURW ptr"
 
+definition
+  sanitise_register :: "tcb \<Rightarrow> register \<Rightarrow> machine_word \<Rightarrow> machine_word"
+where
+  "sanitise_register t r v \<equiv> case r of
+      CPSR \<Rightarrow> (v && 0xf8000000) || 0x150
+    | _    \<Rightarrow> v"
+
 end
 end
